[experiments] Add some more arithmetic operations

src/Experiments/SimplyTypedArithmetic.v
@@ -20,9 +20,11 @@ Import ListNotations. Local Open Scope Z_scope.
 
 Definition runtime_mul := Z.mul.
 Definition runtime_add := Z.add.
+Definition runtime_opp := Z.opp.
 Delimit Scope runtime_scope with RT.
 Infix "*" := runtime_mul : runtime_scope.
 Infix "+" := runtime_add : runtime_scope.
+Notation "- a" := (runtime_opp a%RT) : runtime_scope.
 
 Module Associational.
   Definition eval (p:list (Z*Z)) : Z :=
@@ -54,6 +56,12 @@ Module Associational.
   Lemma eval_mul p q : eval (mul p q) = eval p * eval q.
   Proof. induction p; cbv [mul]; push; nsatz.                 Qed.
   Hint Rewrite eval_mul : push_eval.
+
+  Definition negate_snd (p:list (Z*Z)) : list (Z*Z) :=
+    map (fun cx => (fst cx, (-snd cx)%RT)) p.
+  Lemma eval_negate_snd p : eval (negate_snd p) = - eval p.
+  Proof. induction p; cbv [negate_snd]; push; nsatz.          Qed.
+  Hint Rewrite eval_negate_snd : push_eval.
 
   Example base10_2digit_mul (a0:Z) (a1:Z) (b0:Z) (b1:Z) :
     {ab| eval ab = eval [(10,a1);(1,a0)] * eval [(10,b1);(1,b0)]}.
@@ -93,15 +101,11 @@ Module Associational.
   Hint Rewrite eval_reduce : push_eval.
 
   Section Carries.
-    Context {modulo div : Z -> Z -> Z}.
-    Context {div_mod : forall a b:Z, b <> 0 ->
-                                     a = b * (div a b) + modulo a b}.
-
     Definition carryterm (w fw:Z) (t:Z * Z) :=
       if (Z.eqb (fst t) w)
       then dlet_nd t2 := snd t in
-           dlet_nd d2 := div t2 fw in
-           dlet_nd m2 := modulo t2 fw in
+           dlet_nd d2 := Z.div t2 fw in
+           dlet_nd m2 := Z.modulo t2 fw in
            [(w * fw, d2);(w,m2)]
       else [t].
 
@@ -109,7 +113,7 @@ Module Associational.
       eval (carryterm w fw t) = eval [t].
     Proof using Type*.
       cbv [carryterm Let_In]; break_match; push; [|trivial].
-      specialize (div_mod (snd t) fw fw_nonzero).
+      pose proof (Z.div_mod (snd t) fw fw_nonzero).
       rewrite Z.eqb_eq in *.
       nsatz.
     Qed. Hint Rewrite eval_carryterm using auto : push_eval.
@@ -139,8 +143,9 @@ Module Positional. Section Positional.
   (* SKIP over this: zeros, add_to_nth *)
   Local Ltac push := autorewrite with push_eval push_map distr_length
     push_flat_map push_fold_right push_nth_default cancel_pair natsimplify.
-  Definition zeros n : list Z
-    := List.repeat 0 n.
+  Definition zeros n : list Z := List.repeat 0 n.
+  Lemma length_zeros n : length (zeros n) = n. Proof. cbv [zeros]; distr_length. Qed.
+  Hint Rewrite length_zeros : distr_length.
   Lemma eval_zeros n : eval n (zeros n) = 0.
   Proof.
     cbv [eval Associational.eval to_associational zeros].
@@ -202,6 +207,9 @@ Module Positional. Section Positional.
   Hint Rewrite @eval_from_associational : push_eval.
 
   Section mulmod.
+    (** TODO(for jadep, from jgross): Add a comment about why we take
+        in [m] rather than just using [s - Associational.eval c], or
+        just remove [m] *)
     Context (m:Z) (m_nz:m <> 0) (s:Z) (s_nz:s <> 0)
             (c:list (Z*Z)) (Hm:m = s - Associational.eval c).
     Definition mulmod (n:nat) (a b:list Z) : list Z
@@ -219,14 +227,47 @@ Module Positional. Section Positional.
     induction c as [|?? IHc]; simpl; trivial.                 Qed.
   End mulmod.
 
-  Section Carries.
-    Context {modulo div: Z -> Z -> Z}.
-    Context {div_mod : forall a b:Z, b <> 0 ->
-                                     a = b * (div a b) + modulo a b}.
+  Section add.
+    Context (m:Z) (m_nz:m <> 0) (s:Z) (s_nz:s <> 0)
+            (c:list (Z*Z)) (Hm:m = s - Associational.eval c).
+    Definition add (n:nat) (a b:list Z) : list Z
+      := let a_a := to_associational n a in
+         let b_a := to_associational n b in
+         from_associational n (a_a ++ b_a).
+    Lemma eval_add n (f g:list Z)
+          (Hf : length f = n) (Hg : length g = n) :
+      eval n (add n f g) mod m = (eval n f + eval n g) mod m.
+    Proof. cbv [add]; rewrite Hm in *; push; trivial.
+    destruct n; auto.                                         Qed.
+  End add.
 
+  Section sub.
+    (** TODO(jadep): Fill me in *)
+    Axiom sub : forall (n:nat) (a b:list Z), list Z. (* should be balanced *)
+    Axiom eval_sub
+      : forall (s:Z)
+               (c:list (Z*Z))
+               n (f g:list Z)
+               (Hf : length f = n) (Hg : length g = n),
+        eval n (sub n f g) mod (s - Associational.eval c)
+        = (eval n f - eval n g) mod (s - Associational.eval c).
+    Hint Rewrite eval_sub : push_eval.
+    Definition opp (n:nat) (a:list Z) : list Z
+      := sub n (zeros n) a.
+    Lemma eval_opp
+          (s:Z)
+          (c:list (Z*Z))
+          n (f:list Z)
+          (Hf : length f = n)
+      : eval n (opp n f) mod (s - Associational.eval c)
+        = (- eval n f) mod (s - Associational.eval c).
+    Proof. cbv [opp]; push; distr_length.                     Qed.
+  End sub.
+
+  Section Carries.
     Definition carry {n m} (index:nat) (p:list Z) : list Z :=
       from_associational
-        m (@Associational.carry modulo div (weight index)
+        m (@Associational.carry (weight index)
                                 (weight (S index) / weight index)
                                 (to_associational n p)).
 
@@ -276,6 +317,18 @@ Module Positional. Section Positional.
         destruct n; intros; push; auto.
     Qed. Hint Rewrite @eval_chained_carries : push_eval.
 
+    (* Reverse of [eval]; translate from Z to basesystem by putting
+    everything in first digit and then carrying. *)
+    Definition encode {n} s c (x : Z) : list Z :=
+      chained_carries (n:=n) s c (from_associational n [(1,x)]) (seq 0 n).
+    Lemma eval_encode {n} s c x :
+      (s <> 0) -> (s - Associational.eval c <> 0) -> (n <> 0%nat) ->
+      (forall i, In i (seq 0 n) -> weight (S i) / weight i <> 0) ->
+      eval n (@encode n s c x) mod (s - Associational.eval c)
+      = x mod (s - Associational.eval c).
+    Proof using Type*. cbv [encode]; intros; push; auto; f_equal; omega. Qed.
+    Hint Rewrite @eval_encode : push_eval.
+
   End Carries.
 
 
@@ -305,8 +358,8 @@ Module Positional. Section Positional.
       erewrite <-eval_mulmod with (s:=s) (c:=c)
         by (subst; try assumption; try reflexivity).
       etransitivity;
-        [ | rewrite <- @eval_chained_carries with (s:=s) (c:=c) (idxs:=idxs) (modulo:=fun x y => Z.modulo x y) (div:=fun x y => Z.div x y)
-            by (subst; try assumption; auto using Z.div_mod); reflexivity ].
+        [ | rewrite <- @eval_chained_carries with (s:=s) (c:=c) (idxs:=idxs)
+            by (subst; auto); reflexivity ].
       eapply f_equal2; [|trivial]. eapply f_equal.
       expand_lists ().
       subst carry_mulmod.
